---
title: 'STA 601/360 Homework1'
author: "Jae Hyun Lee, jl914"
date: "`r format(Sys.time(), '%d %B, %Y')`"
output: 
  html_document:
    theme: cerulean
    highlight: tango
---

```{r setup, message=F, warning=F, echo=F}
library(tidyverse)
require(magrittr)
require(plyr)
ggplot2::theme_set(ggplot2::theme_bw())
knitr::opts_chunk$set(fig.align = 'center')
```

# HW1 for STA-601


## Exercise 1
Full conditionals: Let X,Y,Z be random variables with joint density

$$
p(x,y,z) \propto f(x,z)g(y,z)h(z)
$$
Show that 

### part (a) 
$$
p(x \mid y,z) \propto f(x,z)
$$
answer: 
$$
p(x,y,z) = p(x \mid y,z) \times p(y \mid z) \times p(z) \propto f(x,z)g(y,z),h(z)
$$ 
Obviously 
$$ p(z) \propto h(z) $$ 
and 
$$p(y \mid z) = p(y,z) / p(z)$$ 
$$\rightarrow  p(y,z) \propto g(y,z) 
\rightarrow p(y \mid z) \propto g(y,z) 
$$ Thus remaining 
$$ p(x \mid y,z) \propto f(x,z) $$ 

### part (b) 
$$
p(y \mid x,z) \propto g(y,z)
$$
answer: 
$$
p(x,y,z) = p(y \mid x,z) \times p(x \mid z) \times p(z) \propto f(x,z)g(y,z),h(z)
$$ 
Obviously 
$$ p(z) \propto h(z)
$$ 
and 
$$p(x \mid z) = p(x,z) / p(z)
$$ 
$$
\rightarrow  p(x,z) \propto f(x,z) 
\rightarrow p(x \mid z) \propto f(x,z) 
$$ Thus remaining 
$$ p(y \mid x,z) \propto g(y,z) 
$$ 

### part(c\) 
X and Y are conditionally independent given Z
answer: 
By definition, if X and Y are independent,
$$ p(x,y \mid z) = p(x \mid z)p(y \mid z) $$ and it implies that
$$ p(x \mid y,z) = p(x \mid z) \;or\; p(y \mid x,z) = p(y \mid z) $$ As shown at above questions, I could find that their full conditional distribution do not depend on each other
$$ p(x \mid y,z) \propto f(x,z) \propto p(x \mid z) $$
$$ p(y \mid x,z) \propto g(y,z) \propto p(y \mid z) $$   
Thus I can conclude that they are conditional independent.




## Exercise 2
conditional independence: show that 

$$ A^{c} \perp B, A \perp B^{c}, A^{c} \perp B^{c}
\quad  if \quad A \perp B$$


### part(a)
If A,B are conditionally independent given C then
$$ p(A \cap B \mid C) = p(A \mid C)p(B \mid C)$$ Then

<!-- How to use aligned environment in LaTeX -->
$$
\begin{aligned}
p(A^{c} \cap B \mid C) &= p(B \mid C) - p(A \cap B \mid C) \\ 
&= p(B \mid C) - p(A \mid C)p(B \mid C) \\ 
&= p(B \mid C)[1 - p(A \mid C)] \\
&= p(B \mid C)p(A^{c} \mid C)
\end{aligned}
$$

Similarly 

$$
\begin{aligned}
p(A \cap B^{c} \mid C) &= p(A \mid C) - p(A \cap B \mid C) \\
&= p(A \mid C) - p(A \mid C)p(B \mid C) \\ 
&= p(A \mid C)[1 - p(B \mid C)] \\
&= p(A \mid C)p(B^{c} \mid C)
\end{aligned}
$$

Lastly,

$$ 
\begin{aligned}
p(A^{c} \cap B^{c} \mid C) &= p((A \cup B)^{c} \mid C) \\
&= 1- p(A \cup B \mid C) \\
&= 1 - [p(A \mid C) + p(B \mid C) - p(A \cap B \mid C)]\\
&= 1 - p(A \mid C) - p(B \mid C) + p(B \mid C)p(A \mid C) \\
&= [1-p(A \mid C)][1-p(B \mid C)] \\
&= p(A^{c} \mid C)p(B^{c} \mid C)
\end{aligned}
$$



### part(b)

show the example that 
$$ A \perp B \mid C \quad hold \quad A \perp B \mid C^{c} \quad not \; hold  $$
Let consider 2 fair dice toss and event A,B,C are as below:     
* A = first dice value is 1      
* B = second dice value is 1      
* C = sum of dice is less or equal to 2     

Then we can find probability functions of A,B,C as follow:     
$$ p(A \mid C) = 1, p(B \mid C) = 1, p(A \cap B \mid C) =1 \rightarrow A \perp B \mid C $$ and
$$ p(A \mid C^{c}) =5/35, p(B \mid C^{c}) = 5/35, p(A \cap B \mid C^{c}) = 0/35 \\ \rightarrow A \perp B \mid C^{c} \;does \; not \; hold$$

## Exercise 3
There are three coins in a bag; two fair coins (probability of heads = probability of tails) and one fake coin (probability of heads = 1).  
a. You reach in and select one coin at random and throw it in the air. What is the probability that it lands on heads?  
b. You reach in and select one coin at random and throw it in the air and get heads. What is the probability that it is the fake coin?

Let $A$ be the event that I choose fair coin and $A^{c}$ is event that I choose fake coin.     
Then, $p(A)$ = 2/3, $p(A^{c})$ = 1/3   
When Z is event that I have head, $p(Z \mid A)$ = 1/2, $p(Z \mid A^{c})$ = 1   

### part(a)
$$ p(Z) =p(Z \mid A)p(A) + p(Z \mid A^{c})p(A^{c}) = 1/3 + 1/3 = 2/3 $$

### part(b)
$$
\begin{aligned}
p(A^{c} \mid Z) &= p(A^{c} \cap Z) /p(Z) \\
&= p(Z \mid A^{c})p(A^{c})/p(Z) \\
&= 1/3 \,/ \, 2/3 = 1/2 
\end{aligned}
$$ 


## Exercise4
Monty Hall Problem! There are three doors on stage and a host hides a prize behind one of the doors and goats behind the other two doors. A contestant picks one of the three doors (say door 1) and then the game show host opens one of the remaining two doors (say door 3), making sure to reveal a goat. Should the contestant switch to door 2?  
Prior knowledge: The prize originally had 1/3 probability of being behind any of the three doors.  
The host's model: he knows which door has the prize. If he has to choose between a door with a goat and one with a prize, he chooses the one with the prize. If he has to choose between two doors with goats, he picks one of the doors with probability 1/2.

### answer:
Organize situation as A, B, C are event that prize is behind each door 1,2,3 and E is event that game host show goat in door 3.    
$p(A),p(B),p(C)$ = 1/3 for each event.    
If prize is in door1, host choose two doors with probability 1/2. 
Thus $p(E \mid A)$ = 1/2.   
In the case that prize is in door2, host have to choose between goat and prize in above situation. Following the host's model, I think there is typo, so I changed rule from original that he should show prize between prize and goat to modified one that he should show goat between prize and goat.      
So he cannot open door2 and $p(E \mid B)$ = 1.     
If prize is in door3, he cannot show goat at door3 then $p(E \mid C)$ = 0.   
Thus $p(E) = p(E \mid A)p(A) + p(E \mid B)p(B) = 1/2$ and $\,p(A \mid E)=1/3, p(B \mid E)=2/3$    
Consequently, since given E, probability of B is higher than A, contester should change his decision.    